

# Convex MDPs

## 1 Preliminaries

The convex MDP problem can be written as

$$\min_{d_\pi \in \mathcal{K}} f(d_\pi),$$

where  $f : \Delta(\mathcal{A} \mid \mathcal{S}) \mapsto \mathbb{R}$  is a convex function,  $d_\pi \in \Delta(\mathcal{A} \mid \mathcal{S})$  is the state-action stationary distribution induced by policy  $\pi$ , and  $\mathcal{K}$  is the set consisting of all the admissible occupancy measures. The objective can be equivalently written using Fenchel duality as

$$\begin{aligned} \min_{d_\pi \in \mathcal{K}} f(d_\pi) &\stackrel{(i)}{=} \min_{d_\pi \in \mathcal{K}} f^{**}(d_\pi) \\ &\stackrel{(ii)}{=} \min_{d_\pi \in \mathcal{K}} \max_{\lambda \in \Lambda} (\langle \lambda, d_\pi \rangle - f^*(\lambda)) \\ &\stackrel{(iii)}{=} \max_{\lambda \in \Lambda} \min_{d_\pi \in \mathcal{K}} (\langle \lambda, d_\pi \rangle - f^*(\lambda)). \end{aligned}$$

(i) follows that the biconjugate  $f^{**} := f^*(f) = f$  if  $f$  is convex and lower semicontinuous. (ii) follows the definition of Fenchel conjugate:  $f^*(x) := \sup_y x \cdot y - f(y)$ , and  $\Lambda$  is the closure of the (sub-)gradient space  $\{\partial f(d_\pi) \mid d_\pi \in \mathcal{K}\}$ . (iii) follows from the minmax theorem.

Therefore, we can define the Lagrangian as  $\mathcal{L}(d_\pi, \lambda) := \langle \lambda, d_\pi \rangle - f^*(\lambda)$ .

## 2 Linear Function Approximation

We can tackle the above formulation with a primal-dual learning framework. Suppose we can run the algorithm for  $K$  iterations, and for each iteration  $k \in [K]$ , we have that

$$\begin{aligned} d_\pi^k &= \arg \min_{d_\pi \in \mathcal{K}} \langle \lambda^k, d_\pi \rangle, \\ \lambda^k &= \arg \max_{\lambda \in \Lambda} \left\langle \lambda, \sum_{j=1}^k d_\pi^j \right\rangle - k \cdot f^*(\lambda). \end{aligned}$$

**Dual-Variable Parameterization.** Assume that the dual variable  $\lambda$  can be parameterized by a linear function. That is,  $\lambda_\theta = \langle \phi, \theta \rangle$  where  $\phi : \mathcal{S} \times \mathcal{A} \mapsto \mathbb{R}^d$  is the feature map, and  $\theta : \mathbb{R}^d$  is the learnable parameter.

Given the above parameterization, we can rewrite the dual update as follows. Note that in the discounted setting,  $d_\pi(s, a) = (1 - \gamma) \mathbb{E}_\pi[\sum_{t=1}^\infty \gamma^t \mathbb{1}(s_t = s, a_t = a)]$ . Then, we have that

$$\begin{aligned} \lambda^k &= \arg \max_{\lambda \in \Lambda} \left\langle \lambda, \sum_{j=1}^k d_\pi^j \right\rangle - k \cdot f^*(\lambda) \\ &= \arg \max_{\theta \in \mathbb{R}^d} \sum_{s,a} \lambda_\theta(s, a) \cdot \sum_{j=1}^k d_\pi^j(s, a) - k \cdot f^*(\langle \phi, \theta \rangle) \end{aligned}$$

$$\begin{aligned}
&= \arg \max_{\theta \in \mathbb{R}^d} \sum_{j=1}^k \sum_{s,a} \lambda_{\theta}(s,a) \cdot d_{\pi}^j(s,a) - k \cdot f^*(\langle \phi, \theta \rangle) \\
&= \arg \max_{\theta \in \mathbb{R}^d} \sum_{j=1}^k \left\langle \sum_{s,a} d_{\pi}^j(s,a) \cdot \phi(s,a), \theta \right\rangle - k \cdot f^*(\langle \phi, \theta \rangle) \\
&= \arg \max_{\theta \in \mathbb{R}^d} (1 - \gamma) \sum_{j=1}^k \left\langle \sum_{s,a} \mathbb{E}_{\pi_j} \left[ \sum_{t=1}^{\infty} \gamma^t \mathbb{1}(s_t = s, a_t = a) \right] \cdot \phi(s,a), \theta \right\rangle - k \cdot f^*(\langle \phi, \theta \rangle) \\
&= \arg \max_{\theta \in \mathbb{R}^d} (1 - \gamma) \sum_{j=1}^k \left\langle \mathbb{E}_{\pi_j} \left[ \sum_{t=1}^{\infty} \gamma^t \phi(s_t, a_t) \right], \theta \right\rangle - k \cdot f^*(\langle \phi, \theta \rangle)
\end{aligned}$$

We can then use sampling-based approach to estimate  $\mathbb{E}_{\pi_j} [\sum_{t=1}^{\infty} \gamma^t \phi(s_t, a_t)]$  using  $\pi_j$  where  $\pi_j(s, a) = \frac{d_{\pi}^j(s, a)}{\sum_{a'} d_{\pi}^j(s, a')}$ .

### 3 Exploration

## References

## Contents of Appendix